\documentclass{article}
\usepackage{amsmath} % For math equations
\usepackage{amsfonts} % For math fonts
\usepackage{amssymb} % For math symbols
\usepackage{enumitem}
\setlist[enumerate,1]{label=\arabic*.}
\setlist[enumerate,2]{label=\alph*.,itemindent=2em}

\title{part 3}
\author{Asher Christian 006-150-286}
\date{2024-05-28}

\begin{document}
    \maketitle
    \section{Discrete}
    $X$ : eye color of random person\\
    $Y$ : hair\\
    $N(x,y) = \#$ of people of eye color $x$ and hair color $y$ \\
    $p(x,y) = P(X = x , Y = y) = \frac{N(x,y)}{N}$ \\
    $N =$ total \#\\
    $N(x) = \sum_{y}N(x,y)$ \\
    $N(x,\cdot) = \sum_{y}^{}N(x,y)$\\ 
    $N(\cdot,y) = \sum_{x}^{}N(x,y)$ \\
    \[
    p(x) = P(X=x) = \frac{N(x, \cdot)}{N} = \frac{\sum_{y}^{}N(x,y)}{N} = \sum_{y}^{}\frac{N(x,y)}{N} = \sum_{y}^{}p(x,y)
    .\] 
    \[
    p(y) = \sum_{x}^{}p(x,y)
    .\] 
   \\\\
   Conditional:
   \[
       p(y|x) = P(X=x | Y = y) = \frac{N(x,y)}{N(\cdot ,y)} = (\frac{\frac{N(x,y)}{N}}{\frac{N(\cdot ,y)}{N}}) = \frac{p(x,y)}{p(y)}
   .\] 
   \[
   p(y|x) = \frac{p(x,y)}{p(x)}
   .\] 
   \[
   p(x,y) = p(x)p(y|x) = p(y)p(x|y)
   .\] 
   \[
   p(x|y) = \frac{p(x,y)}{p(y)} = \frac{p(x,y)}{\sum_{x}^{}p(x,y)} = \frac{p(x)p(y|x)}{\sum_{x}^{}p(x)p(y|x)}
   .\] 
   \[
   p(y) = \sum_{x}^{}p(x,y) = \sum_{x}^{}p(x)p(y|x)
   .\] 
   \[
   E(h(x)) = \sum_{x}^{}h(x)p(x)
   .\] 
   \[
   E(h(x,y)) = \sum_{x}^{}\sum_{y}^{}h(x,y)p(x,y) = \sum_{x, y}^{}h(x,y) \frac{N(x,y)}{N} = \frac{1}{N} \sum_{x,y}^{}h(x,y)N(x,y)
   .\] 
   The population average of h\\\\
   Continuous random variables\\
   $X$ = height of random person\\
   $Y$ = weight\\

   \[
       f(x,y) = \frac{\text{\# of points in} (x, x+\Delta x) \cdot  (y, y + \Delta y) / N}{\Delta x\Delta y  } = \frac{P(X \in (x, x + \Delta x) \&  Y \in (y, y + \Delta y))}{\Delta x\Delta y  }  
   .\]    
   \[
   = \frac{\frac{N(x,y)}{N}}{\Delta x\Delta y  }
   .\] 
   \begin{align*}
       f(x) &= \frac{\text{Proportion}}{\text{size}}\\
            &= \frac{N(X,\cdot ) / N}{\Delta x } \\
            &= \frac{P(X \in (x, x+\Delta x))}{\Delta x } \\
            &= \frac{\sum_{y}^{}\frac{N(x,y)}{N}}{\Delta x }\\
            &= \frac{\sum_{y}^{}f(x,y)\Delta x\Delta y}{\Delta x }\\
            &= \sum_{y}^{}f(x,y)\Delta y \\
            &= \int_{}^{}f(x,y)dy
   \end{align*}
   \[
   f(y) = \int_{}^{}f(x,y)dx
   .\] 
   Conditional
   \begin{align*}
       f(x|y) &= \frac{\text{Proportion}}{\text{Size}}\\
              &= \frac{P(X \in (x, x+\Delta x)| Y \in (y,y+\Delta y )}{\Delta x }\\
              &= \frac{\frac{N(x,y)}{N(\cdot ,y)}}{\Delta x }\\
              &= \frac{\frac{N(x,y)}{N} / \frac{N(\cdot ,y)}{N}}{\Delta x }\\
              &= \frac{\frac{f(x,y)\Delta x\Delta y}{f(y)\Delta y }}{\Delta x }\\
              &= \frac{f(x,y)}{f(y)}
   \end{align*}
   \begin{align*}
       f(x,y) &= f(x)f(y|x) \\
              &= f(y)f(x|y)
   \end{align*}
   \begin{align*}
       E(h(x,y)) &= \int_{x}^{}\int_{y}^{}h(x,y)f(x,y)dxdy\\
                 &= \frac{1}{N} \sum_{x}^{}\sum_{y}^{}h(x,y)N(x,y)
   \end{align*}
   $p(x,y)$ prob mass function or probability desnity function\\
   Rule 1: Marginalization
    \begin{align*}
        p(x) &= \sum_{y}^{}p(x,y)\\
             &= \int_{}^{}p(x,y)dy\\
        p(y) &= \sum_{x}^{}p(x,y)\\
             &= \int_{}^{}p(x,y)dx
   \end{align*}
   Rule 2: Conditioning
   \begin{align*}
       p(x|y) &= \frac{p(x,y)}{p_y(y)}\\
       p(y|x) &= \frac{p(x,y)}{P_x(x)}\\
   \end{align*}
   Rule 3: Chain
   \begin{align*}
       P(x,y) &= p(x)p(y|x) \\
              &= P(y)p(x|y)
   \end{align*}
   Independence $X$ orthogonal $Y$ 
   \[
   P(x,y) = p_x(x)p_y(y), p(x|y) = p_x(x), p(y|x) = p_y(y)
   .\] 
   \section{Day 2}
   \[
   E(h(x,y)) = \int_{y}^{}\int_{x}^{}h(x,y)f(x,y)dxdy
   .\] 
   independence:
   \[
   p(x,y) = p_x(x)p_y(y)
   .\] 
   Standardization\\
   $\mu $ = $E(x), \sigma^2=Var(x), X <- \frac{x-\mu }{\sigma }$
   \[
   X \sim N(0,1)
   .\] 
   \begin{align*}
       f_x(x) = \frac{1}{\sqrt{2\pi }}e^{-\frac{x^2}{2}}
   \end{align*}
   \[
       [Y|X=x] \sim N(\rho x, 1- \rho^2) \text{  regression model}
   .\] 
   \[
   f(Y|x) = \frac{1}{\sqrt{2\pi (1-\rho^2)}}e^{\frac{-(y-\rho x)^2}{2(1-\rho^2)}}
   .\] 
   $\rho < 1$
   $y = \rho x$ is the regression line
   \begin{enumerate}
       \item Conditional expectation \& variance\\
           $E(Y|X = x) = \rho x$\\
            $Var(Y|X = x) = 1-\rho^2$ regression towards the mean\\
            $Y = \rho X + \epsilon $ and epsilon is indep of  $x$\\
            $\epsilon \sim N(0, 1-\rho^2)$ $\epsilon $ is independant of $X$\\
            $Y = \rho x + \epsilon  \sim N(\rho x, 1- \rho^2)$ \\
            $E(Y) = E(\rho X + \epsilon ) = \rho E(x) + E(\epsilon ) = \rho$\\
            $Var(Y) = Var(\rho X) + Var(\epsilon ) = \rho^2Var(X) + (1-\rho^2) = 1$
        \item Modern meaning of regression
            $E(Y|X) = f(x)$ 
        \item 
            \[
                (x,y) \sim f(x,y)
            .\] 
            \[
            Cov(x,y) = E((X-E(X))(Y-E(Y))
            .\] 
            \[
            Cov(x,x) = E((X-E(X))^2) = Var(X)
            .\] 
            Covariance changes units depending on the measure - to fix that we standardize\\
            \[
                Cov(\frac{X-\mu_X}{\sigma_X}, \frac{Y-\mu_Y}{\sigma_Y}) = E((X_{s})(Y_{s}))
            .\] 
            \[
            = \frac{E((X-\mu _X)(Y-\mu_Y))}{\sigma _X\sigma _Y} = \frac{Cov(X,Y)}{\sqrt{Var(X)}\sqrt{Var(Y)}} 
            .\] 
            \[
            = \rho = Corr(X,Y)
            .\] 
            

   \end{enumerate}

\end{document}
